feat: Add API skeleton for DynamoDBEncryption (#4)
* feat: Add API skeleton for DynamoDBEncryption and include minimal
integration with the Structured Encryption Library

src/StructuredEncryption/src/Index.dfy
@@ -1,7 +1,7 @@
 // Copyright Amazon.com Inc. or its affiliates. All Rights Reserved.
 // SPDX-License-Identifier: Apache-2.0
 include "../../../private-aws-encryption-sdk-dafny-staging/src/StandardLibrary/StandardLibrary.dfy"
-include "../Model/AwsCryptographyStructuredEncryptionTypes.dfy"
+include "../model/AwsCryptographyStructuredEncryptionTypes.dfy"
 include "Operations/EncryptStructureOperation.dfy"
 include "Operations/DecryptStructureOperation.dfy"
 
@@ -75,14 +75,30 @@ module
 
     method EncryptStructure(input: Types.EncryptStructureInput)
         returns (output: Result<Types.EncryptStructureOutput, Types.Error>)
-      requires ValidState()
-      modifies Modifies - {History},
-        History`EncryptStructure
-      decreases Modifies ,
+      requires
+        && ValidState()
+        && (
+          input.keyring.Some? ==>
+            && input.keyring.value.ValidState()
+            && input.keyring.value.Modifies !! Modifies
+        ) && (
+          input.cmm.Some? ==>
+            && input.cmm.value.ValidState()
+            && input.cmm.value.Modifies !! Modifies
+        )
+      modifies
+        Modifies - {History},
+        History`EncryptStructure,
+        (if input.keyring.Some? then input.keyring.value.Modifies else {}),
+        (if input.cmm.Some? then input.cmm.value.Modifies else {})
+      decreases
+        Modifies,
         (if input.keyring.Some? then input.keyring.value.Modifies else {}) ,
         (if input.cmm.Some? then input.cmm.value.Modifies else {})
+      ensures
+        && ValidState()
       ensures EncryptStructureEnsuresPublicly(input, output)
-      ensures History.EncryptStructure == old(History.EncryptStructure) + [Types.DafnyCallEvent(input, output)]
+      ensures History.EncryptStructure == old(History.EncryptStructure) + [DafnyCallEvent(input, output)]
     {
       output := EncryptStructureOperation.EncryptStructure(config, input);
       History.EncryptStructure := History.EncryptStructure + [Types.DafnyCallEvent(input, output)];
@@ -90,14 +106,30 @@ module
 
     method DecryptStructure(input: Types.DecryptStructureInput)
         returns (output: Result<Types.DecryptStructureOutput, Types.Error>)
-      requires ValidState()
-      modifies Modifies - {History},
-        History`DecryptStructure
-      decreases Modifies ,
-        (if input.keyring.Some? then input.keyring.value.Modifies else {}) ,
+      requires
+        && ValidState()
+        && (
+          input.keyring.Some? ==>
+            && input.keyring.value.ValidState()
+            && input.keyring.value.Modifies !! Modifies
+        ) && (
+          input.cmm.Some? ==>
+            && input.cmm.value.ValidState()
+            && input.cmm.value.Modifies !! Modifies
+        )
+      modifies
+        Modifies - {History},
+        History`DecryptStructure,
+        (if input.keyring.Some? then input.keyring.value.Modifies else {}),
         (if input.cmm.Some? then input.cmm.value.Modifies else {})
+      decreases
+        Modifies,
+        (if input.keyring.Some? then input.keyring.value.Modifies else {}),
+        (if input.cmm.Some? then input.cmm.value.Modifies else {})
+      ensures
+        && ValidState()
       ensures DecryptStructureEnsuresPublicly(input, output)
-      ensures History.DecryptStructure == old(History.DecryptStructure) + [Types.DafnyCallEvent(input, output)]
+      ensures History.DecryptStructure == old(History.DecryptStructure) + [DafnyCallEvent(input, output)]
     {
       output := DecryptStructureOperation.DecryptStructure(config, input);
       History.DecryptStructure := History.DecryptStructure + [Types.DafnyCallEvent(input, output)];
