src/StructuredEncryption/src/Operations/EncryptStructureOperation.dfy
@@ -1,7 +1,7 @@
 // Copyright Amazon.com Inc. or its affiliates. All Rights Reserved.
 // SPDX-License-Identifier: Apache-2.0
 include "../../../../private-aws-encryption-sdk-dafny-staging/src/StandardLibrary/StandardLibrary.dfy"
-include "../../Model/AwsCryptographyStructuredEncryptionTypes.dfy"
+include "../../model/AwsCryptographyStructuredEncryptionTypes.dfy"
 include "../StructuredEncryptionConstants.dfy"
 
 module EncryptStructureOperation {
