Makefile
@@ -1,26 +1,57 @@
 ROOT_DIR:=$(shell dirname $(realpath $(firstword $(MAKEFILE_LIST))))
 DYLD_LIBRARY_PATH=$(DYLD_LIBRARY_PATH)
 
-verify: verify_structured_encryption
-
-verify_structured_encryption:
-	$(MAKE) -C src/StructuredEncryption verify
+####
+# Build Targets
+####
 
 build: build_dotnet
 
-test: test_dotnet
-
-build_dotnet: build_dotnet_structured_encryption
+build_dotnet: build_dotnet_structured_encryption build_dotnet_ddb_encryption
 
 build_dotnet_structured_encryption:
 	$(MAKE) -C src/StructuredEncryption build_dotnet
 
-test_dotnet: test_dotnet_structured_encryption
+build_dotnet_ddb_encryption:
+	$(MAKE) -C src/DynamoDBEncryption build_dotnet
+
+####
+# Verify Targets
+####
+
+verify: verify_structured_encryption verify_ddb_encryption
+
+verify_structured_encryption:
+	$(MAKE) -C src/StructuredEncryption verify
+
+verify_ddb_encryption:
+	$(MAKE) -C src/DynamoDBEncryption verify
+
+####
+# Test Targets
+####
+
+test: test_dotnet
+
+test_dotnet: test_dotnet_structured_encryption test_dotnet_ddb_encryption
 
 test_dotnet_structured_encryption:
 	$(MAKE) -C src/StructuredEncryption test_dotnet
 
-generate_models: generate_models_structured_encryption
+test_dotnet_ddb_encryption:
+	$(MAKE) -C src/DynamoDBEncryption test_dotnet
+
+####
+# Generate Models Targets
+####
+
+generate_models: generate_models_structured_encryption generate_models_ddb_encryption generate_models_aws_ddb
 
 generate_models_structured_encryption:
 	$(MAKE) -C src/StructuredEncryption generate_models
+
+generate_models_ddb_encryption:
+	$(MAKE) -C src/DynamoDBEncryption generate_models
+
+generate_models_aws_ddb:
+	$(MAKE) -C src/AWS-DDB generate_models
