README.md
@@ -35,7 +35,7 @@ you may encounter an error that says:
 make generate-models
 ```
 
-Generates new models using the polymorph submodule.
+Generates new models for the Structured Encryption Library, DDBEC, and DDB using the polymorph submodule.
 Will overwrite models, but will not clean up old models that are not overwritten.
 
 ### Verify Dafny Code
